Finish verification of saturn/mpmc_queue_1.

theories/saturn/mpmc_queue_1.v
@@ -4,23 +4,26 @@
 
 From zoo Require Import
   prelude.
+From zoo.common Require Import
+  list.
 From zoo.iris.base_logic Require Import
   lib.mono_list
+  lib.auth_nat_max
   lib.twins.
 From zoo.language Require Import
   notations
   diaframe.
 From zoo.std Require Import
   option
-  node2_schain
-  node2_chain.
+  node2_schain.
 From zoo.saturn Require Export
   base.
 From zoo Require Import
   options.
 
+Implicit Types b strong : bool.
 Implicit Types l front node back new_back : location.
-Implicit Types past nodes : list location.
+Implicit Types hist past nodes : list location.
 Implicit Types v t : val.
 Implicit Types vs : list val.
 
@@ -40,7 +43,7 @@ Definition mpmc_queue_create : val :=
 
 Definition mpmc_queue_is_empty : val :=
   λ: "t",
-    "t".{front}.{node2_next} = ().
+"t".{front}.{node2_next} = ().
 
 #[local] Definition mpmc_queue_do_push : val :=
   rec: "mpmc_queue_do_push" "node" "new_back" :=
@@ -48,7 +51,7 @@ Definition mpmc_queue_is_empty : val :=
     if: "node'" = () then (
       ifnot: Cas "node".[node2_next] () "new_back" then (
         Yield ;;
-        "mpmc_queue_do_push" "node'" "new_back"
+  "mpmc_queue_do_push" "node" "new_back"
       )
     ) else (
       "mpmc_queue_do_push" "node'" "new_back"
@@ -72,24 +75,24 @@ Definition mpmc_queue_pop : val :=
     let: "front" := "old_front".{node2_next} in
     if: "front" = () then (
       §None
-    ) else (
-      if: Cas "t".[front] "old_front" "front" then (
+    ) else if: Cas "t".[front] "old_front" "front" then (
         let: "v" := "front".{node2_data} in
         "front" <-{node2_data} () ;;
         ‘Some{ "v" }
-      ) else (
-        Yield ;;
-        "mpmc_queue_pop" "t"
-      )
+    ) else (
+      Yield ;;
+      "mpmc_queue_pop" "t"
     ).
 
 Class MpmcQueueG Σ `{zoo_G : !ZooG Σ} := {
   #[local] mpmc_queue_G_history_G :: MonoListG Σ location ;
+  #[local] mpmc_queue_G_front_G :: AuthNatMaxG Σ ;
   #[local] mpmc_queue_G_model_G :: TwinsG Σ (leibnizO (list val)) ;
 }.
 
 Definition mpmc_queue_Σ := #[
   mono_list_Σ location ;
+  auth_nat_max_Σ ;
   twins_Σ (leibnizO (list val))
 ].
 #[global] Instance subG_mpmc_queue_Σ Σ `{zoo_G : !ZooG Σ} :
@@ -104,6 +107,7 @@ Section mpmc_queue_G.
 
   Record mpmc_queue_meta := {
     mpmc_queue_meta_history : gname ;
+    mpmc_queue_meta_front : gname ;
     mpmc_queue_meta_model : gname ;
   }.
 
@@ -114,10 +118,12 @@ Section mpmc_queue_G.
   Proof.
     pose encode γ := (
       γ.(mpmc_queue_meta_history),
+      γ.(mpmc_queue_meta_front),
       γ.(mpmc_queue_meta_model)
     ).
-    pose decode := λ '(γ_history, γ_model), {|
+    pose decode := λ '(γ_history, γ_front, γ_model), {|
       mpmc_queue_meta_history := γ_history ;
+      mpmc_queue_meta_front := γ_front ;
       mpmc_queue_meta_model := γ_model ;
     |}.
     refine (inj_countable' encode decode _). intros []. done.
@@ -130,6 +136,13 @@ Section mpmc_queue_G.
   #[local] Definition mpmc_queue_history_elem γ i node :=
     mono_list_elem γ.(mpmc_queue_meta_history) i node.
 
+  #[local] Definition mpmc_queue_front_auth' γ_front i :=
+    auth_nat_max_auth γ_front (DfracOwn 1) i.
+  #[local] Definition mpmc_queue_front_auth γ i :=
+    mpmc_queue_front_auth' γ.(mpmc_queue_meta_front) i.
+  #[local] Definition mpmc_queue_front_lb γ i :=
+    auth_nat_max_lb γ.(mpmc_queue_meta_front) i.
+
   #[local] Definition mpmc_queue_model₁' γ_model vs :=
     twins_twin1 γ_model (DfracOwn 1) vs.
   #[local] Definition mpmc_queue_model₁ γ vs :=
@@ -140,13 +153,15 @@ Section mpmc_queue_G.
     mpmc_queue_model₂' γ.(mpmc_queue_meta_model) vs.
 
   #[local] Definition mpmc_queue_inv_inner l γ : iProp Σ :=
-    ∃ past front nodes back vs,
-    ⌜back ∈ past ++ front :: nodes⌝ ∗
+    ∃ hist past front nodes back vs,
+    ⌜hist = past ++ front :: nodes⌝ ∗
+    ⌜back ∈ hist⌝ ∗
     l.[front] ↦ #front ∗
     l.[back] ↦ #back ∗
-    node2_schain (past ++ [front]) (from_option #@{location} ()%V $ head nodes) ∗
-    node2_chain nodes vs () ∗
-    mpmc_queue_history_auth γ (past ++ front :: nodes) ∗
+    node2_schain hist () ∗
+    ([∗ list] node; v ∈ nodes; vs, node.[node2_data] ↦ v) ∗
+    mpmc_queue_history_auth γ hist ∗
+    mpmc_queue_front_auth γ (length past) ∗
     mpmc_queue_model₂ γ vs.
   Definition mpmc_queue_inv t ι : iProp Σ :=
     ∃ l γ,
@@ -199,6 +214,34 @@ Section mpmc_queue_G.
     apply mono_list_update_app.
   Qed.
 
+  #[local] Lemma mpmc_queue_front_alloc :
+    ⊢ |==>
+      ∃ γ_front,
+      mpmc_queue_front_auth' γ_front 0.
+  Proof.
+    apply auth_nat_max_alloc.
+  Qed.
+  #[local] Lemma mpmc_queue_front_lb_get γ i :
+    mpmc_queue_front_auth γ i ⊢
+    mpmc_queue_front_lb γ i.
+  Proof.
+    apply auth_nat_max_lb_get.
+  Qed.
+  #[local] Lemma mpmc_queue_front_lb_valid γ i1 i2 :
+    mpmc_queue_front_auth γ i1 -∗
+    mpmc_queue_front_lb γ i2 -∗
+    ⌜i2 ≤ i1⌝.
+  Proof.
+    apply auth_nat_max_lb_valid.
+  Qed.
+  #[local] Lemma mpmc_queue_front_update {γ i} i' :
+    i ≤ i' →
+    mpmc_queue_front_auth γ i ⊢ |==>
+    mpmc_queue_front_auth γ i'.
+  Proof.
+    apply auth_nat_max_update.
+  Qed.
+
   #[local] Lemma mpmc_queue_model_alloc :
     ⊢ |==>
       ∃ γ_model,
@@ -240,10 +283,12 @@ Section mpmc_queue_G.
     wp_record l as "Hmeta" "(Hl_front & Hl_back & _)".
 
     iMod mpmc_queue_history_alloc as "(%γ_history & Hhistory_auth)".
+    iMod mpmc_queue_front_alloc as "(%γ_front & Hfront_auth)".
     iMod mpmc_queue_model_alloc as "(%γ_model & Hmodel₁ & Hmodel₂)".
 
     pose γ := {|
       mpmc_queue_meta_history := γ_history ;
+      mpmc_queue_meta_front := γ_front ;
       mpmc_queue_meta_model := γ_model ;
     |}.
 
@@ -251,27 +296,122 @@ Section mpmc_queue_G.
 
     iApply "HΦ".
     iSplitR "Hmodel₁"; last iSteps.
-    iStep 2. iApply inv_alloc. iExists [], front, [], front, []. iFrame. iSteps.
-    - rewrite elem_of_list_singleton //.
-    - iApply node2_chain_nil.
+    iStep 2. iApply inv_alloc.
+    iExists [front], [], front, [], front, []. iFrame. iSteps.
+    rewrite elem_of_list_singleton //.
   Qed.
 
-  Lemma mpmc_queue_is_empty_spec t ι :
-    <<<
-      mpmc_queue_inv t ι
-    | ∀∀ vs,
-      mpmc_queue_model t vs
-    >>>
-      mpmc_queue_is_empty t
-    <<<
-      mpmc_queue_model t vs
-    | RET #(bool_decide (vs = [])); True
-    >>>.
-  Proof.
-  Admitted.
-
-  #[local] Lemma mpmc_queue_node2_next_spec l ι γ i node :
+  #[local] Lemma mpmc_queue_front_spec l γ ι :
     {{{
+      inv ι (mpmc_queue_inv_inner l γ)
+    }}}
+      !#l.[front]
+    {{{ front i,
+      RET #front;
+      mpmc_queue_history_elem γ i front ∗
+      mpmc_queue_front_lb γ i
+    }}}.
+  Proof.
+    iIntros "%Φ #Hinv HΦ".
+
+    iInv "Hinv" as "(%hist & %past & %front & %nodes & %back & %vs & >%Hhist & >%Hback & Hl_front & Hl_back & Hhist & Hnodes & Hhistory_auth & Hfront_auth & Hmodel₂)".
+    wp_load.
+    iDestruct (mpmc_queue_history_elem_get _ front with "Hhistory_auth") as "#Hhistory_elem".
+    { rewrite Hhist list_lookup_middle //. }
+    iDestruct (mpmc_queue_front_lb_get with "Hfront_auth") as "#Hfront_lb".
+    iSplitR "HΦ". { repeat iExists _. iSteps. }
+    iSteps.
+  Qed.
+
+  #[local] Lemma mpmc_queue_back_spec l γ ι :
+    {{{
+      inv ι (mpmc_queue_inv_inner l γ)
+    }}}
+      !#l.[back]
+    {{{ back i,
+      RET #back;
+      mpmc_queue_history_elem γ i back
+    }}}.
+  Proof.
+    iIntros "%Φ #Hinv HΦ".
+
+    iInv "Hinv" as "(%hist & %past & %front & %nodes & %back & %vs & >%Hhist & >%Hback & Hl_front & Hl_back & Hhist & Hnodes & Hhistory_auth & Hfront_auth & Hmodel₂)".
+    wp_load.
+    pose proof Hback as (i & Hlookup)%elem_of_list_lookup.
+    iDestruct (mpmc_queue_history_elem_get with "Hhistory_auth") as "#Hhistory_elem_back"; first done.
+    iSplitR "HΦ". { repeat iExists _. iSteps. }
+    iSteps.
+  Qed.
+
+  #[local] Lemma mpmc_queue_node2_next_spec_strong strong TB β Ψ l γ ι i node :
+    {{{
+      meta l nroot γ ∗
+      inv ι (mpmc_queue_inv_inner l γ) ∗
+      mpmc_queue_history_elem γ i node ∗
+      if strong then
+        mpmc_queue_front_lb γ i ∗
+        atomic_update (TA := [tele vs]) (TB := TB) (⊤ ∖ ↑ι) ∅ (tele_app $ mpmc_queue_model #l) β Ψ ∗
+        (mpmc_queue_model #l [] -∗ ∃ x, β [tele_arg []] x)
+      else
+        True
+    }}}
+      !#node.[node2_next]
+    {{{ res,
+      RET res;
+      ( ⌜res = ()%V⌝ ∗
+        if strong then
+          ∃ x, Ψ [tele_arg []] x
+        else
+          True
+      ) ∨ (
+        ∃ node',
+        ⌜res = #node'⌝ ∗
+        mpmc_queue_history_elem γ (S i) node' ∗
+        if strong then
+          atomic_update (TA := [tele vs]) (TB := TB) (⊤ ∖ ↑ι) ∅ (tele_app $ mpmc_queue_model #l) β Ψ
+        else
+          True
+      )
+    }}}.
+  Proof.
+    iIntros "%Φ (#Hmeta & #Hinv & #Hhistory_elem & HΨ) HΦ".
+
+    iInv "Hinv" as "(%hist & %past & %front & %nodes & %back & %vs & >%Hhist & >%Hback & Hl_front & Hl_back & Hhist & Hnodes & >Hhistory_auth & Hfront_auth & Hmodel₂)".
+    iDestruct (mpmc_queue_history_agree with "Hhistory_auth Hhistory_elem") as %Hlookup.
+    iDestruct (node2_schain_lookup with "Hhist") as "(Hnode & Hhist)"; first done.
+    wp_load.
+    iDestruct ("Hhist" with "Hnode ") as "Hhist".
+    destruct (hist !! S i) as [node' |] eqn:Hlookup'; simpl.
+
+    - iDestruct (mpmc_queue_history_elem_get (S i) with "Hhistory_auth") as "#Hhistory_elem'"; first done.
+      iSplitR "HΨ HΦ". { repeat iExists _. iSteps. }
+      destruct strong; iSteps.
+
+    - destruct strong.
+
+      + iDestruct "HΨ" as "(#Hfront_lb & HΨ & Hβ)".
+        iDestruct (mpmc_queue_front_lb_valid with "Hfront_auth Hfront_lb") as %Hi.
+        destruct (decide (length vs = 0)) as [->%nil_length_inv | Hvs]; last first.
+        { iDestruct (big_sepL2_length with "Hnodes") as %?.
+          exfalso.
+          apply (f_equal length) in Hhist.
+          opose proof* lookup_last_length as Heq; [done.. |].
+          rewrite Heq app_length /= in Hhist. lia.
+        }
+        iMod "HΨ" as "(%vs & (%_l & %_γ & %Heq & #_Hmeta & Hmodel₁) & _ & HΨ)". injection Heq as <-.
+        iDestruct (meta_agree with "Hmeta _Hmeta") as %<-. iClear "_Hmeta".
+        iDestruct (mpmc_queue_model_agree with "Hmodel₁ Hmodel₂") as %->.
+        iDestruct ("Hβ" with "[Hmodel₁]") as "(%x & Hβ)"; first iSteps.
+        iMod ("HΨ" with "Hβ") as "HΨ".
+        iSplitR "HΨ HΦ". { repeat iExists _. iSteps. }
+        iSteps.
+
+      + iSplitR "HΦ". { repeat iExists _. iSteps. }
+        iSteps.
+  Qed.
+  #[local] Lemma mpmc_queue_node2_next_spec l γ ι i node :
+    {{{
+      meta l nroot γ ∗
       inv ι (mpmc_queue_inv_inner l γ) ∗
       mpmc_queue_history_elem γ i node
     }}}
@@ -284,30 +424,64 @@ Section mpmc_queue_G.
         mpmc_queue_history_elem γ (S i) node'
     }}}.
   Proof.
-    iIntros "%Φ (#Hinv & #Hhistory_elem) HΦ".
+    iIntros "%Φ (#Hmeta & #Hinv & #Hhistory_elem) HΦ".
+    wp_apply (mpmc_queue_node2_next_spec_strong false TeleO inhabitant inhabitant with "[$]").
+    iSteps.
+  Qed.
 
-    iInv "Hinv" as "(%past & %front & %nodes & %back & %vs & >%Hback & Hl_front & Hl_back & >Hpast & Hnodes & >Hhistory_auth & Hmodel₂)".
-    iDestruct (mpmc_queue_history_agree with "Hhistory_auth Hhistory_elem") as
-      %[Hlookup | (_ & [(_ & <-) | (_ & Hlookup)]%lookup_cons_Some)]%lookup_app_Some.
+  Lemma mpmc_queue_is_empty_spec t ι :
+    <<<
+      mpmc_queue_inv t ι
+    | ∀∀ vs,
+      mpmc_queue_model t vs
+    >>>
+      mpmc_queue_is_empty t @ ↑ι
+    <<<
+      ∃∃ b,
+      mpmc_queue_model t vs
+    | RET #b;
+      if b then ⌜vs = []⌝ else True
+    >>>.
+  Proof.
+    iIntros "!> %Φ (%l & %γ & -> & #Hmeta & #Hinv) HΦ".
 
-    - wp_apply (node2_next_spec_schain_lookup with "Hpast") as "Hpast".
-      { apply lookup_app_l_Some. done. }
-      assert (∃ node', (past ++ [front]) !! S i = Some node') as (node' & Hlookup').
-      { destruct (decide (S i = length past)).
-        - rewrite list_lookup_middle //. naive_solver.
-        - rewrite list_lookup_lookup_total_lt; last naive_solver.
-          apply lookup_lt_Some in Hlookup. rewrite app_length. lia.
+    wp_rec.
+    wp_smart_apply (mpmc_queue_front_spec with "Hinv") as (front i) "(#Hhistory_elem & #Hfront_lb)".
+    wp_pures.
+
+    wp_bind (!_)%E.
+    rename front into node.
+    iInv "Hinv" as "(%hist & %past & %front & %nodes & %back & %vs & >%Hhist & >%Hback & Hl_front & Hl_back & Hhist & Hnodes & >Hhistory_auth & Hfront_auth & Hmodel₂)".
+    iDestruct (mpmc_queue_history_agree with "Hhistory_auth Hhistory_elem") as %Hlookup.
+    iDestruct (node2_schain_lookup with "Hhist") as "(Hnode & Hhist)"; first done.
+    wp_load.
+    iDestruct ("Hhist" with "Hnode ") as "Hhist".
+    destruct (hist !! S i) as [node' |] eqn:Hlookup'; simpl.
+
+    - iMod "HΦ" as "(%_vs & (%_l & %_γ & %Heq & #_Hmeta & Hmodel₁) & _ & HΦ)". injection Heq as <-.
+      iDestruct (meta_agree with "Hmeta _Hmeta") as %<-. iClear "_Hmeta".
+      iDestruct (mpmc_queue_model_agree with "Hmodel₁ Hmodel₂") as %->.
+      iMod ("HΦ" $! false with "[Hmodel₁] [//]") as "HΦ"; first iSteps.
+      iSplitR "HΦ". { repeat iExists _. iSteps. }
+      iSteps.
+
+    - iDestruct (mpmc_queue_front_lb_valid with "Hfront_auth Hfront_lb") as %Hi.
+      destruct (decide (length vs = 0)) as [->%nil_length_inv | Hvs]; last first.
+      { iDestruct (big_sepL2_length with "Hnodes") as %?.
+        exfalso.
+        apply (f_equal length) in Hhist.
+        opose proof* lookup_last_length as Heq; [done.. |].
+        rewrite Heq app_length /= in Hhist. lia.
       }
-      iDestruct (mpmc_queue_history_elem_get (S i) with "Hhistory_auth") as "#Hhistory_elem'".
-      { rewrite (assoc _ _ [_]). apply lookup_app_l_Some. done. }
-      rewrite Hlookup' /=. iSteps.
+      iMod "HΦ" as "(%vs & (%_l & %_γ & %Heq & #_Hmeta & Hmodel₁) & _ & HΦ)". injection Heq as <-.
+      iDestruct (meta_agree with "Hmeta _Hmeta") as %<-. iClear "_Hmeta".
+      iDestruct (mpmc_queue_model_agree with "Hmodel₁ Hmodel₂") as %->.
+      iMod ("HΦ" $! true with "[Hmodel₁] [//]") as "HΦ"; first iSteps.
+      iSplitR "HΦ". { repeat iExists _. iSteps. }
+      iSteps.
+  Qed.
 
-    - admit.
-
-    - admit.
-  Admitted.
-
-  #[local] Lemma mpmc_queue_do_push_spec l ι γ i node new_back v :
+  #[local] Lemma mpmc_queue_do_push_spec l γ ι i node new_back v :
     <<<
       meta l nroot γ ∗
       inv ι (mpmc_queue_inv_inner l γ) ∗
@@ -329,13 +503,44 @@ Section mpmc_queue_G.
     iLöb as "HLöb" forall (i node) "Hhistory_elem".
 
     wp_rec.
-    wp_smart_apply (mpmc_queue_node2_next_spec with "[$Hinv $Hhistory_elem]") as (res) "[-> | (%node' & -> & #Hhistory_elem')]"; last iSteps.
+    wp_smart_apply (mpmc_queue_node2_next_spec with "[$Hmeta $Hinv $Hhistory_elem]") as (res) "[-> | (%node' & -> & #Hhistory_elem')]"; last iSteps.
     wp_pures.
 
     wp_bind (Cas _ _ _).
-    admit.
-  Admitted.
-  #[local] Lemma mpmc_queue_fix_back_spec l ι γ i back j new_back :
+    iInv "Hinv" as "(%hist & %past & %front & %nodes & %back & %vs & >%Hhist & >%Hback & Hl_front & Hl_back & Hhist & Hnodes & >Hhistory_auth & Hfront_auth & Hmodel₂)".
+    iDestruct (mpmc_queue_history_agree with "Hhistory_auth Hhistory_elem") as %Hlookup.
+    iDestruct (node2_schain_lookup' with "Hhist") as "(Hhist1 & Hnode & Hhist2)"; first done.
+    destruct (hist !! S i) as [node' |] eqn:Hlookup'; simpl.
+
+    - wp_cas as _ | [] _.
+      iDestruct (node2_schain_lookup'_2 with "Hhist1 Hnode Hhist2") as "Hhist"; [done | rewrite Hlookup' // |].
+      iSplitR "Hnew_back HΦ". { repeat iExists _. iSteps. }
+      iSteps.
+
+    - wp_cas as Hcas | _ _; first done.
+      iDestruct (node2_schain_lookup'_2 with "Hhist1 Hnode []") as "Hhist"; [done | rewrite Hlookup' // | ..].
+      { rewrite -(lookup_last_length hist) // drop_all //. }
+      iDestruct "Hnew_back" as "(Hnew_back_data & Hnew_back_next)".
+      iDestruct (big_sepL2_snoc with "[$Hnodes $Hnew_back_data]") as "Hnodes".
+      iDestruct (node2_schain_snoc_2 with "Hhist Hnew_back_next") as "Hhist".
+      iMod (mpmc_queue_history_update new_back with "Hhistory_auth") as "Hhistory_auth".
+      iDestruct (mpmc_queue_history_elem_get with "Hhistory_auth") as "#Hhistory_elem_new_back".
+      { rewrite lookup_snoc_Some. naive_solver. }
+      iMod "HΦ" as "(%_vs & (%_l & %_γ & %Heq & #_Hmeta & Hmodel₁) & _ & HΦ)". injection Heq as <-.
+      iDestruct (meta_agree with "Hmeta _Hmeta") as %<-. iClear "_Hmeta".
+      iDestruct (mpmc_queue_model_agree with "Hmodel₁ Hmodel₂") as %->.
+      iMod (mpmc_queue_model_update (vs ++ [v]) with "Hmodel₁ Hmodel₂") as "(Hmodel₁ & Hmodel₂)".
+      iMod ("HΦ" with "[Hmodel₁]") as "HΦ"; [iSteps.. |].
+      iSplitR "HΦ".
+      { iExists (hist ++ [new_back]), past, front, (nodes ++ [new_back]), back, (vs ++ [v]).
+        iSteps; iPureIntro.
+        - rewrite Hhist -assoc //.
+        - rewrite elem_of_app. naive_solver.
+      }
+      iSteps.
+  Qed.
+
+  #[local] Lemma mpmc_queue_fix_back_spec l γ ι i back j new_back :
     {{{
       meta l nroot γ ∗
       inv ι (mpmc_queue_inv_inner l γ) ∗
@@ -349,11 +554,26 @@ Section mpmc_queue_G.
   Proof.
     iIntros "%Φ (#Hmeta & #Hinv & #Hhistory_elem_back & #Hhistory_elem_new_back) HΦ".
 
-    iLöb as "HLöb".
+    iLöb as "HLöb" forall (i back) "Hhistory_elem_back".
 
-    wp_rec.
-    admit.
-  Admitted.
+    wp_rec. wp_pures.
+    wp_bind (_ and _)%E.
+    wp_apply (wp_wand _ _ (λ res, ∃ b, ⌜res = #b⌝)%I) as (res) "(%b & ->)".
+    { wp_smart_apply (mpmc_queue_node2_next_spec with "[$Hmeta $Hinv $Hhistory_elem_new_back]") as (res) "[-> | (%new_back' & -> & #Hhistory_elem_new_back')]"; last iSteps.
+      wp_pures.
+
+      wp_bind (Cas _ _ _).
+      iInv "Hinv" as "(%hist & %past & %front & %nodes & %back' & %vs & >%Hhist & >%Hback & Hl_front & Hl_back & Hhist & Hnodes & Hhistory_auth & Hfront_auth & Hmodel₂)".
+      wp_cas as _ | -> _.
+      2: iDestruct (mpmc_queue_history_agree with "Hhistory_auth Hhistory_elem_new_back") as %Hnew_back%elem_of_list_lookup_2.
+      all: iSplitL; first (repeat iExists _; iSteps).
+      all: iSteps.
+    }
+    destruct b; last iSteps.
+    wp_smart_apply (mpmc_queue_back_spec with "Hinv") as (back' i') "#Hhistory_elem_back'".
+    iApply ("HLöb" with "HΦ Hhistory_elem_back'").
+  Qed.
+
   Lemma mpmc_queue_push_spec t ι v :
     <<<
       mpmc_queue_inv t ι
@@ -370,19 +590,9 @@ Section mpmc_queue_G.
 
     wp_rec.
     wp_smart_apply (node2_create_spec with "[//]") as (new_back) "Hnew_back".
-    wp_pures.
-
-    wp_bind (!_)%E.
-    iInv "Hinv" as "(%past & %front & %nodes & %back & %vs & >%Hback & Hfront & Hback & Hpast & Hnodes & Hhistory_auth & Hmodel₂)".
-    wp_load.
-    pose proof Hback as (i & Hlookup)%elem_of_list_lookup.
-    iDestruct (mpmc_queue_history_elem_get with "Hhistory_auth") as "#Hhistory_elem_back"; first done.
-    iSplitR "Hnew_back HΦ"; first iSteps.
-    iModIntro. clear.
-
+    wp_smart_apply (mpmc_queue_back_spec with "Hinv") as (back i) "#Hhistory_elem_back".
     wp_smart_apply (mpmc_queue_do_push_spec with "[$Hmeta $Hinv $Hhistory_elem_back $Hnew_back]").
     iApply (atomic_update_wand with "HΦ"). iIntros "%vs HΦ (%j & #Hhistory_elem_new_back)".
-
     wp_smart_apply (mpmc_queue_fix_back_spec with "[$Hmeta $Hinv Hhistory_elem_back Hhistory_elem_new_back] HΦ").
     iSteps.
   Qed.
@@ -399,7 +609,46 @@ Section mpmc_queue_G.
     | RET head vs; True
     >>>.
   Proof.
-  Admitted.
+    iIntros "!> %Φ (%l & %γ & -> & #Hmeta & #Hinv) HΦ".
+
+    iLöb as "HLöb".
+
+    wp_rec.
+    wp_smart_apply (mpmc_queue_front_spec with "Hinv") as (old_front i) "(#Hhistory_elem_old & #Hfront_lb_old)".
+    wp_smart_apply (mpmc_queue_node2_next_spec_strong true with "[$Hmeta $Hinv $Hhistory_elem_old $Hfront_lb_old $HΦ]") as (res) "[(-> & (% & HΦ)) | (%front & -> & #Hhistory_elem & HΦ)]"; [iSmash.. |].
+    wp_pures.
+
+    wp_bind (Cas _ _ _).
+    iInv "Hinv" as "(%hist & %past & %front' & %nodes & %back & %vs & >%Hhist & >%Hback & Hl_front & Hl_back & Hhist & Hnodes & >Hhistory_auth & Hfront_auth & Hmodel₂)".
+    iDestruct (mpmc_queue_history_agree with "Hhistory_auth Hhistory_elem") as %Hlookup.
+    iDestruct (node2_schain_lookup with "Hhist") as "(Hnode & Hhist)"; first done.
+    wp_cas as _ | [= ->] _.
+    all: iDestruct ("Hhist" with "Hnode ") as "Hhist".
+
+    - iSplitR "HΦ". { repeat iExists _. iSteps. }
+      iSteps.
+
+    - iDestruct (mpmc_queue_history_agree with "Hhistory_auth Hhistory_elem_old") as %Hlookup_old.
+      iAssert ⌜length past = i⌝%I as %Hlength.
+      { iDestruct (node2_schain_NoDup with "Hhist") as %Hnodup.
+        iPureIntro. eapply NoDup_lookup; try done.
+        rewrite Hhist list_lookup_middle //.
+      }
+      rewrite Hhist (assoc _ _ [_]) lookup_app_r app_length /= in Hlookup; first lia.
+      rewrite Nat.add_1_r Hlength Nat.sub_diag in Hlookup.
+      destruct nodes as [| node nodes]; first done. injection Hlookup as ->.
+      rewrite (assoc _ _ [_]) in Hhist.
+      iDestruct (big_sepL2_cons_inv_l with "Hnodes") as "(%v & %vs' & -> & Hfront_data & Hnodes)".
+      iMod (mpmc_queue_front_update (length (past ++ [old_front])) with "Hfront_auth") as "Hfront_auth".
+      { rewrite app_length. lia. }
+      iMod "HΦ" as "(%_vs & (%_l & %_γ & %Heq & #_Hmeta & Hmodel₁) & _ & HΦ)". injection Heq as <-.
+      iDestruct (meta_agree with "Hmeta _Hmeta") as %<-. iClear "_Hmeta".
+      iDestruct (mpmc_queue_model_agree with "Hmodel₁ Hmodel₂") as %->.
+      iMod (mpmc_queue_model_update vs' with "Hmodel₁ Hmodel₂") as "(Hmodel₁ & Hmodel₂)".
+      iMod ("HΦ" with "[Hmodel₁]") as "HΦ"; first iSteps.
+      iSplitR "Hfront_data HΦ". { repeat iExists _. iSteps. }
+      iSteps.
+  Qed.
 End mpmc_queue_G.
 
 #[global] Opaque mpmc_queue_create.
